correctness/RegexCorrectness/Backtracker/Compile.lean
@@ -10,32 +10,11 @@ open Regex.Data (BitMatrix BoundedIterator)
 
 namespace Regex.Backtracker
 
-theorem captureNext.go.path_done_of_some {nfa wf startIdx maxIdx bit update} {visited visited' : BitMatrix nfa.nodes.size (maxIdx + 1 - startIdx)}
-  (v : bit.Valid) (hres : captureNext.go HistoryStrategy nfa wf startIdx maxIdx bit visited = (.some update, visited')) :
-  ∃ state it it', it'.toString = bit.it.toString ∧ nfa[state] = .done ∧ Path nfa wf it it' state update := by
-  induction bit, visited using captureNext.go.induct' HistoryStrategy nfa wf startIdx with
-  | found bit visited update' visited' haux =>
-    simp [captureNext.go_found haux] at hres
-    simp [hres] at haux
-    have ⟨l, r, vf⟩ := (bit.valid_of_valid v).validFor
-    have inv₀ : captureNextAux.StackInv wf bit [⟨[], ⟨nfa.start, wf.start_lt⟩, bit⟩] := by
-      simp [captureNextAux.StackInv]
-      exact .init (bit.valid_of_valid v)
-    have ⟨state, it, hn, path⟩ := captureNextAux.path_done_of_some haux inv₀
-    exact ⟨state, bit.it, it, by rw [path.toString_eq], hn, path⟩
-  | not_found_next bit visited visited' haux hnext ih =>
-    simp [captureNext.go_not_found_next haux hnext] at hres
-    exact ih (bit.next_valid hnext v) hres
-  | not_found_end bit visited visited' haux hnext => simp [captureNext.go_not_found_end haux hnext] at hres
-
 theorem captureNext.path_done_of_some {nfa wf it update} (hres : captureNext HistoryStrategy nfa wf it = .some update) (v : it.Valid) :
   ∃ state it' it'', it''.toString = it.toString ∧ nfa[state] = .done ∧ Path nfa wf it' it'' state update := by
   if le : it.pos ≤ it.toString.endPos then
     simp [captureNext_le le] at hres
-    let result := go HistoryStrategy nfa wf it.pos.byteIdx it.toString.endPos.byteIdx ⟨it, (Nat.le_refl _), le, rfl⟩ (BitMatrix.zero _ _)
-    change result.1 = .some update at hres
-    have : result = (.some update, result.2) := by simp [Prod.ext_iff, hres]
-    exact captureNext.go.path_done_of_some (BoundedIterator.valid_of_it_valid v) this
+    exact captureNext.go.path_done_of_some (BoundedIterator.valid_of_it_valid v) hres
   else
     simp [captureNext_not_le le] at hres
 
